App compat

ctx-equiv-ixfree/lang.v
@@ -24,7 +24,7 @@ Inductive expr :=
   (* | bind (e1 : expr) (x : binder) (e2 : expr) *)
   | app (e1 e2: expr)
   (* | abs (x : binder) (e : expr) *)
-  | eplus (e1 e2: expr)
+  (* | eplus (e1 e2: expr) *)
 
 with val :=
   | vint (z : Z)
@@ -66,7 +66,7 @@ with subst (x : string) (es : expr) (e : expr)  : expr :=
   (* | abs y e =>
       abs y $ if decide (BNamed x = y) then e else subst x es e *)
   | app e1 e2 => app (subst x es e1) (subst x es e2)
-  | eplus e1 e2 => eplus (subst x es e1) (subst x es e2)
+  (* | eplus e1 e2 => eplus (subst x es e1) (subst x es e2) *)
   end.
 
 Definition subst' (mx : binder) (es : expr) : expr → expr :=
@@ -101,32 +101,74 @@ Inductive base_step : expr → expr → Prop :=
      base_step (Plus e1 e2) (eint n3) *)
   .
 
+(* inside-out contexts *)
+(* https://www.williamjbowman.com/teaching/2020/w1/cpsc509/resources/05-reduction.pdf *)
 Inductive ectx :=
-  | HoleCtx
-  | AppLCtx (K: ectx) (v2 : val)
-  | AppRCtx (e1 : expr) (K: ectx)
-  | PlusLCtx (K: ectx) (v2 : val)
-  | PlusRCtx (e1 : expr) (K: ectx)
-  .
+| ectx_hole   : ectx
+| ectx_app1   : ectx → expr → ectx
+| ectx_app2   : val → ectx → ectx
+.
 
-Fixpoint fill (K : ectx) (e : expr) : expr :=
-  match K with
-  | HoleCtx => e
-  | AppLCtx K v2 => app (fill K e) (of_val v2)
-  | AppRCtx e1 K => app e1 (fill K e)
-  | PlusLCtx K v2 => eplus (fill K e) (of_val v2)
-  | PlusRCtx e1 K => eplus e1 (fill K e)
+Fixpoint plug (E : ectx) (e : expr) : expr :=
+  match E with
+  | ectx_hole       => e
+  | ectx_app1 E1 e1  => plug E1 (app e e1)
+  | ectx_app2 v E1   => plug E1 (app v e)
   end.
 
-(* filling a context with another context *)
-Fixpoint comp_ectx (Ko Ki: ectx) :=
-  match Ko with
-  | HoleCtx => Ki
-  | AppLCtx K v2 => AppLCtx (comp_ectx K Ki) v2
-  | AppRCtx e1 K => AppRCtx e1 (comp_ectx K Ki)
-  | PlusLCtx K v2 => PlusLCtx (comp_ectx K Ki) v2
-  | PlusRCtx e1 K => PlusRCtx e1 (comp_ectx K Ki)
+(** Outside-in evaluation contexts *)
+Inductive rctx :=
+| rctx_hole   : rctx
+| rctx_app1   : rctx → expr → rctx
+| rctx_app2   : val → rctx → rctx
+.
+
+Fixpoint rplug (E : rctx) (e : expr) : expr :=
+  match E with
+  | rctx_hole       => e
+  | rctx_app1 E1 e1  => app (rplug E1 e) e1
+  | rctx_app2 v E1   => app v (rplug E1 e)
   end.
+
+
+(* these behave the same *)
+Compute plug ectx_hole vunit.
+Compute plug (ectx_app1 ectx_hole (vint 2)) (vint 1).
+
+(*
+  assuming 2 is the innermost application, ((1 2) 3),
+
+  // outside-in contexts
+
+    □[□ 3][□ 2]
+  = (□ 3)[□ 2]
+  = ((□ 2) 3)
+
+  rplug ((□ 2) 3) 1
+  = ((rplug (□ 2) 1) 3)
+  = (((rplug □ 1) 2) 3)
+  = ((1 2) 3)
+
+  // inside-out contexts.
+  // hole args are the surrounding context,
+  // and the topmost term is the innermost context.
+  // the syntax is the same
+
+  E ::= □ | E e | v E
+
+  plug ((□ 3) 2) 1
+  = plug (□ 3) (1 2)
+  = plug □ ((1 2) 3)
+  = ((1 2) 3)
+*)
+
+Compute plug (ectx_app1 (ectx_app1 ectx_hole (vint 3)) (vint 2))
+  (evalue (vint 1)).
+
+Compute rplug (rctx_app1 (rctx_app1 rctx_hole (vint 3)) (vint 2))
+  (evalue (vint 1)).
+
+Notation fill := plug.
 
 Inductive contextual_step (e1 : expr) (e2 : expr) : Prop :=
   Ectx_step K e1' e2' :
@@ -151,47 +193,6 @@ Definition obs_eqv e1 e2 :=
 Infix "≈" := equiterminate (at level 80, right associativity, only printing).
 Infix "≡obs" := obs_eqv (at level 80, right associativity, only printing).
 
-
-
-(* Section logrel.
-Context `{heapGS Σ}.
-
-(* Definition valO := leibnizO val.
-Definition exprO := leibnizO expr.
-Definition evctxO := leibnizO ectx. *)
-
-(* Definition val_rel := valO -n> valO -n> iProp Σ.
-Definition ctx_rel := evctxO -n> evctxO -n> iProp Σ.
-Definition expr_rel := exprO -n> exprO -n> iProp Σ. *)
-
-Definition val_rel := persistent_pred (val * val) (iPropI Σ).
-Definition expr_rel := persistent_pred (expr * expr) (iPropI Σ).
-Definition evctx_rel := persistent_pred (ectx * ectx) (iPropI Σ).
-
-Definition val_relO := persistent_predO (val * val) (iPropI Σ).
-Definition expr_relO := persistent_predO (expr * expr) (iPropI Σ).
-Definition evctx_relO := persistent_predO (ectx * ectx) (iPropI Σ).
-
-Definition mk_val_rel (pred : (val * val) → iProp Σ) {Pers : ∀ v, Persistent (pred v)} : val_rel :=
-  @PersPred _ _ pred Pers.
-Global Instance val_rel_pers (τ : val_relO) : ∀ v, Persistent (τ v) := _.
-
-Definition mk_expr_rel (pred : (expr * expr) → iProp Σ) {Pers : ∀ e, Persistent (pred e)} : expr_rel :=
-  @PersPred _ _ pred Pers.
-Global Instance expr_rel_pers (τ : expr_relO) : ∀ e, Persistent (τ e) := _.
-
-Definition mk_evctx_rel (pred : (ectx * ectx) → iProp Σ) {Pers : ∀ E, Persistent (pred E)} : evctx_rel :=
-  @PersPred _ _ pred Pers.
-Global Instance evctx_rel_pers (τ : evctx_relO) : ∀ E, Persistent (τ E) := _.
-
-(* Print val_rel_pers. *)
-
-(* Locate "<pers>". *)
-
-(* Definition semtypeO := persistent_predO val (iPropI Σ). *)
-*)
-
-
 Definition sub := gmap string val.
 
 Fixpoint subst_map_val (xs : sub) (v : val) : val :=
@@ -208,7 +209,7 @@ with subst_map (xs : sub) (e : expr) : expr :=
   | var y => match xs !! y with Some es => of_val es | _ =>  var y end
   | app e1 e2 => app (subst_map xs e1) (subst_map xs e2)
   (* | abs x e => abs x (subst_map (binder_delete x xs) e) *)
-  | eplus e1 e2 => eplus (subst_map xs e1) (subst_map xs e2)
+  (* | eplus e1 e2 => eplus (subst_map xs e1) (subst_map xs e2) *)
   end.
 
 Fixpoint is_closed (X : list string) (e : expr) : bool :=
@@ -216,7 +217,9 @@ Fixpoint is_closed (X : list string) (e : expr) : bool :=
   | var x => bool_decide (x ∈ X)
   | evalue vunit | evalue (vint _) => true
   | evalue (vlambda x e) => is_closed (x :b: X) e
-  | app e1 e2 | eplus e1 e2 => is_closed X e1 && is_closed X e2
+  | app e1 e2
+  (* | eplus e1 e2 *)
+  => is_closed X e1 && is_closed X e2
   end.
 Definition closed (X : list string) (e : expr) : Prop := Is_true (is_closed X e).
 
@@ -265,31 +268,31 @@ Definition L_rel_fix := I_fix L_rel_pre.
 Definition L_rel := L_rel_pre L_rel_fix.
 (* Definition L_rel := I_fix L_rel_pre. *)
 
-Definition O_rel e₁ e₂ := L_rel e₁ e₂ ∧ᵢ L_rel e₂ e₁.
+Definition O_rel e1 e2 := L_rel e1 e2 ∧ᵢ L_rel e2 e1.
 
 (* ========================================================================= *)
 
-Lemma L_rel_roll p₁ p₂ n :
-  n ⊨ L_rel p₁ p₂ → n ⊨ L_rel_fix p₁ p₂.
+Lemma L_rel_roll p1 p2 n :
+  n ⊨ L_rel p1 p2 → n ⊨ L_rel_fix p1 p2.
 Proof.
   intro H; iapply (I_fix_roll expr_rel); [ | exact H ].
   apply L_rel_pre_contractive.
 Qed.
 
-Lemma L_rel_unroll p₁ p₂ n :
-  n ⊨ L_rel_fix p₁ p₂ → n ⊨ L_rel p₁ p₂.
+Lemma L_rel_unroll p1 p2 n :
+  n ⊨ L_rel_fix p1 p2 → n ⊨ L_rel p1 p2.
 Proof.
   intro H; iapply (I_fix_unroll expr_rel); [ | exact H ].
   apply L_rel_pre_contractive.
 Qed.
 
-Definition K_rel_pre (V_rel : val_rel) (E₁ E₂ : ectx) :=
+Definition K_rel_pre (V_rel : val_rel) (E1 E2 : ectx) :=
   ∀ᵢ v1 v2 : val,
     (closed [] v1)ᵢ →ᵢ (closed [] v2)ᵢ →ᵢ
-    V_rel v1 v2 →ᵢ O_rel (fill E₁ v1) (fill E₂ v2).
+    V_rel v1 v2 →ᵢ O_rel (fill E1 v1) (fill E2 v2).
 
-Definition R_rel_pre (V_rel : val_rel) (e₁ e₂ : expr) :=
-  ∀ᵢ E₁ E₂, ▷ K_rel_pre V_rel E₁ E₂ →ᵢ O_rel (fill E₁ e₁) (fill E₂ e₂).
+Definition R_rel_pre (V_rel : val_rel) (e1 e2 : expr) :=
+  ∀ᵢ E1 E2, ▷ K_rel_pre V_rel E1 E2 →ᵢ O_rel (fill E1 e1) (fill E2 e2).
 
 Definition V_rel_pre (V_rel : val_rel) : val_rel :=
   λ v1 v2, (closed [] v1)ᵢ →ᵢ (closed [] v2)ᵢ →ᵢ
@@ -316,14 +319,14 @@ Definition G_rel (γ1 γ2 : sub) : IProp :=
     (γ2 !! x = Some v2)ᵢ →ᵢ
     V_rel v1 v2.
 
-Definition E_rel_o (e₁ e₂ : expr) : IProp :=
-  ∀ᵢ γ₁ γ₂, G_rel γ₁ γ₂ →ᵢ E_rel (subst_map γ₁ e₁) (subst_map γ₂ e₂).
+Definition E_rel_o (e1 e2 : expr) : IProp :=
+  ∀ᵢ γ1 γ2, G_rel γ1 γ2 →ᵢ E_rel (subst_map γ1 e1) (subst_map γ2 e2).
 
-Definition V_rel_o (v₁ v₂ : val) : IProp :=
-  ∀ᵢ γ₁ γ₂, G_rel γ₁ γ₂ →ᵢ V_rel (subst_map_val γ₁ v₁) (subst_map_val γ₂ v₂).
+Definition V_rel_o (v1 v2 : val) : IProp :=
+  ∀ᵢ γ1 γ2, G_rel γ1 γ2 →ᵢ V_rel (subst_map_val γ1 v1) (subst_map_val γ2 v2).
 
-(* Definition rel_p (p₁ p₂ : expr) : IProp :=
-  ∀ᵢ γ₁ γ₂, G_rel γ₁ γ₂ →ᵢ O_rel (bind γ₁ p₁) (bind γ₂ p₂). *)
+(* Definition rel_p (p1 p2 : expr) : IProp :=
+  ∀ᵢ γ1 γ2, G_rel γ1 γ2 →ᵢ O_rel (bind γ1 p1) (bind γ2 p2). *)
 
 (* ========================================================================= *)
 (* Contractiveness and urolling fixpoint *)
@@ -333,15 +336,15 @@ Proof.
   intro n; iintros; unfold V_rel_pre, R_rel_pre, K_rel_pre; auto_contr.
 Qed.
 
-Lemma V_rel_roll v₁ v₂ n :
-  n ⊨ V_rel v₁ v₂ → n ⊨ V_rel_fix v₁ v₂.
+Lemma V_rel_roll v1 v2 n :
+  n ⊨ V_rel v1 v2 → n ⊨ V_rel_fix v1 v2.
 Proof.
   intro H; iapply (I_fix_roll val_rel); [ | exact H ].
   apply V_rel_pre_contractive.
 Qed.
 
-Lemma V_rel_unroll v₁ v₂ n :
-  n ⊨ V_rel_fix v₁ v₂ → n ⊨ V_rel v₁ v₂.
+Lemma V_rel_unroll v1 v2 n :
+  n ⊨ V_rel_fix v1 v2 → n ⊨ V_rel v1 v2.
 Proof.
   intro H; iapply (I_fix_unroll val_rel); [ | exact H ].
   apply V_rel_pre_contractive.
@@ -373,39 +376,40 @@ Proof.
   later_shift. apply V_rel_roll. assumption.
 Qed.
 
-Lemma K_rel_intro (E₁ E₂ : ectx) n :
-  n ⊨ (∀ᵢ (v₁ v₂:val), (closed [] v₁)ᵢ →ᵢ (closed [] v₂)ᵢ →ᵢ
-    V_rel v₁ v₂ →ᵢ O_rel (fill E₁ v₁) (fill E₂ v₂)) →
-  n ⊨ K_rel E₁ E₂.
+Lemma K_rel_intro (E1 E2 : ectx) n :
+  n ⊨ (∀ᵢ (v1 v2:val), (closed [] v1)ᵢ →ᵢ (closed [] v2)ᵢ →ᵢ
+    V_rel v1 v2 →ᵢ O_rel (fill E1 v1) (fill E2 v2)) →
+  n ⊨ K_rel E1 E2.
 Proof.
-  intro HE. iintros v₁ v₂ Hcv1 Hcv2 Hv. iapply HE; auto.
+  intro HE. iintros v1 v2 Hcv1 Hcv2 Hv. iapply HE; auto.
   apply V_rel_unroll; assumption.
 Qed.
 
-Lemma K_rel_elim (E₁ E₂ : ectx) (v₁ v₂ : val) n :
-  n ⊨ K_rel E₁ E₂ →
-  n ⊨ (closed [] v₁)ᵢ →
-  n ⊨ (closed [] v₂)ᵢ →
-  n ⊨ V_rel v₁ v₂ →
-  n ⊨ O_rel (fill E₁ v₁) (fill E₂ v₂).
+Lemma K_rel_elim (E1 E2 : ectx) (v1 v2 : val) n :
+  n ⊨ K_rel E1 E2 →
+  n ⊨ (closed [] v1)ᵢ →
+  n ⊨ (closed [] v2)ᵢ →
+  n ⊨ V_rel v1 v2 →
+  n ⊨ O_rel (fill E1 v1) (fill E2 v2).
 Proof.
   intros HE Hc1 Hc2 Hv. iapply HE; auto. apply V_rel_roll; assumption.
 Qed.
 
-Lemma R_rel_elim (e₁ e₂ : expr) E₁ E₂ n :
-  n ⊨ R_rel e₁ e₂ →
-  n ⊨ ▷ K_rel E₁ E₂ →
-  n ⊨ O_rel (fill E₁ e₁) (fill E₂ e₂).
+Lemma R_rel_elim (e1 e2 : expr) E1 E2 n :
+  n ⊨ R_rel e1 e2 →
+  n ⊨ ▷ K_rel E1 E2 →
+  n ⊨ O_rel (fill E1 e1) (fill E2 e2).
 Proof.
   intros He HE; iapply He; assumption.
 Qed.
 
-Lemma E_rel_elim (e₁ e₂ : expr) E₁ E₂ n :
-  n ⊨ E_rel e₁ e₂ →
-  n ⊨ (closed [] e₁)ᵢ →
-  n ⊨ (closed [] e₂)ᵢ →
-  n ⊨ K_rel E₁ E₂ →
-  n ⊨ O_rel (fill E₁ e₁) (fill E₂ e₂).
+(* this is a special case of the bind rule *)
+Lemma E_rel_elim (e1 e2 : expr) E1 E2 n :
+  n ⊨ E_rel e1 e2 →
+  n ⊨ (closed [] e1)ᵢ →
+  n ⊨ (closed [] e2)ᵢ →
+  n ⊨ K_rel E1 E2 →
+  n ⊨ O_rel (fill E1 e1) (fill E2 e2).
 Proof.
   intros He Hc1 Hc2 HE. iapply He; auto.
 Qed.
@@ -419,7 +423,7 @@ Lemma V_rel_elimE (v1 v2 u1 u2 : val) n :
   n ⊨ V_rel u1 u2 →
   n ⊨ E_rel (app v1 u1) (app v2 u2).
 Proof.
-  intros Hv Hcv1 Hcv2 Hcu1 Hcu2 Hu. iintros Hc1 Hc2 E₁ E₂ HE.
+  intros Hv Hcv1 Hcv2 Hcu1 Hcu2 Hu. iintros Hc1 Hc2 E1 E2 HE.
   (* idestruct Hc1. *)
   (* idestruct Hc2. *)
   apply R_rel_elim. 2: { later_shift; assumption. }
@@ -427,64 +431,140 @@ Proof.
   later_shift; assumption.
 Qed.
 
-Lemma compat_val (v₁ v₂ : val) n :
-  n ⊨ V_rel_o v₁ v₂ →
-  n ⊨ E_rel_o v₁ v₂.
+(* val inclusion *)
+Lemma compat_val (v1 v2 : val) n :
+  n ⊨ V_rel_o v1 v2 →
+  n ⊨ E_rel_o v1 v2.
 Proof.
-  intro Hv. iintros γ₁ γ₂ Hγ Hc1 Hc2 E₁ E₂. iintros HE. simpl.
+  intro Hv. iintros γ1 γ2 Hγ Hc1 Hc2 E1 E2. iintros HE. simpl.
   apply K_rel_elim; auto.
   iapply Hv. assumption.
 Qed.
 
-Lemma compat_app (e₁ e₂ e₁' e₂' : expr) n :
-  n ⊨ E_rel_o e₁ e₂ →
-  n ⊨ E_rel_o e₁' e₂' →
-  n ⊨ E_rel_o (app e₁ e₁') (app e₂ e₂').
+Lemma closed_app xs e1 e2:
+  closed xs (app e1 e2) ↔
+  closed xs e1 ∧ closed xs e2.
 Proof.
-  intros He He'.
-  iintros γ₁ γ₂ Hγ E₁ E₂ HE.
-  (* term_simpl. *)
-  (* Check E_rel_intro. *)
-  pose proof E_rel_elim.
-  (* apply E_rel_elim. *)
-  (* apply (E_rel_elim _ _ (AppRCtx _ _) (AppRCtx _ _)). *)
-  (* eapply (E_rel_elim _ _ (AppLCtx _ _) (AppLCtx _ _)). *)
-  (* eapply E_rel_elim with (E₁ := AppRCtx _ _) (E₂ := AppRCtx _ _). *)
-    (* [ *)
-     - simpl.
-
-     Print K_rel_pre.
-     iapply He. assumption.
-      (* | ]. *)
-  apply K_rel_intro; iintros v₁ v₂ Hv.
-  apply E_rel_elim with (E₁ := ectx_app2 _ _) (E₂ := ectx_app2 _ _);
-    [ iapply He'; assumption | ].
-  apply K_rel_intro; iintros u₁ u₂ Hu; simpl.
-  iapply V_rel_elimE; assumption.
+unfold closed. simpl.
+  split.
+  { intros.
+    unfold closed in H.
+    simpl in H.
+    apply andb_prop_elim in H.
+    assumption. }
+  { intros [? ?].
+    unfold closed. simpl.
+    apply andb_prop_intro.
+    firstorder. }
 Qed.
 
-(* Lemma rel_e_compat_callcc {V : Set} (e₁ e₂ : expr (inc V)) n :
-  n ⊨ E_rel e₁ e₂ →
-  n ⊨ E_rel (e_callcc e₁) (e_callcc e₂).
+Lemma compat_app (e1 e2 e1' e2' : expr) n :
+  n ⊨ E_rel_o e1 e2 →
+  n ⊨ E_rel_o e1' e2' →
+  n ⊨ E_rel_o (app e1 e1') (app e2 e2').
+Proof.
+  intros He He'.
+  iintros γ1 γ2 Hγ Hc1 Hc2 E1 E2. iintros HE.
+  simpl.
+  (* this only moves the subs *)
+  pose proof (@E_rel_elim
+    (subst_map γ1 e1)
+    (subst_map γ2 e2)
+    (ectx_app1 E1 (subst_map γ1 e1'))
+    (ectx_app1 E2 (subst_map γ2 e2'))).
+  simpl in H.
+  apply H; clear H.
+  { iapply He. assumption. }
+  { idestruct Hc1.
+    simpl in Hc1.
+    apply closed_app in Hc1.
+    iintro.
+    destruct Hc1.
+    assumption. }
+  { idestruct Hc2.
+    simpl in Hc2.
+    apply closed_app in Hc2.
+    iintro.
+    destruct Hc2.
+    assumption. }
+  { apply K_rel_intro. iintros u₁ u₂ Hcu1 Hcu2 Hu. simpl.
+    apply E_rel_elim with (E1 := ectx_app2 _ _) (E2 := ectx_app2 _ _).
+    { iapply He'. assumption. }
+    {
+      (* TODO look into reflection *)
+      (* Search (_ && _). *)
+      (* Search "reflect". *)
+      idestruct Hc1.
+      iintro.
+      unfold closed in *.
+      (* apply Is_true_reflect. *)
+      simpl in *.
+      auto.
+      simpl in Hc1.
+      apply closed_app in Hc1.
+      destruct Hc1.
+      assumption. }
+    { idestruct Hc2.
+      simpl in Hc2.
+      apply closed_app in Hc2.
+      iintro.
+      destruct Hc2.
+      assumption. }
+    apply K_rel_intro. iintros v1 v2 Hcv1 Hcv2 Hv.
+    simpl.
+    apply E_rel_elim.
+    { apply V_rel_elimE; auto. }
+    { idestruct Hcu1.
+      idestruct Hcv1.
+      iintro. apply closed_app.
+      split; auto. }
+    { idestruct Hcu2.
+      idestruct Hcv2.
+      iintro. apply closed_app.
+      split; auto. }
+    { assumption. } }
+Qed.
+
+Lemma rel_e_compat_app {V : Set} (e1 e2 e1' e2' : expr V) n :
+  n ⊨ rel_e e1 e2 →
+  n ⊨ rel_e e1' e2' →
+  n ⊨ rel_e (e_app e1 e1') (e_app e2 e2').
+Proof.
+  intros He He'.
+  iintros γ1 γ2 Hγ E1 E2 HE; term_simpl.
+  (* apply RelE_elim. *)
+  apply RelE_elim with (E1 := ectx_app1 _ _) (E2 := ectx_app1 _ _).
+    - iapply He; assumption.
+    -
+  apply RelK_intro; iintros v1 v2 Hv.
+  apply RelE_elim with (E1 := ectx_app2 _ _) (E2 := ectx_app2 _ _);
+    [ iapply He'; assumption | ].
+  apply RelK_intro; iintros u1 u2 Hu; simpl.
+  iapply RelV_elimE; assumption.
+Qed.
+
+(* Lemma rel_e_compat_callcc {V : Set} (e1 e2 : expr (inc V)) n :
+  n ⊨ E_rel e1 e2 →
+  n ⊨ E_rel (e_callcc e1) (e_callcc e2).
 Proof.
   intro He.
-  iintros γ₁ γ₂ Hγ E₁ E₂ HE; term_simpl.
+  iintros γ1 γ2 Hγ E1 E2 HE; term_simpl.
   eapply Obs_red_both; [ auto_red | auto_red | ]; later_shift.
   unfold subst; repeat rewrite bind_bind_comp'.
   iapply He; [ | eassumption ].
   iintro x; destruct x as [ | x ]; term_simpl; [ | iapply Hγ ].
-  apply V_rel_intro; iintros u₁ u₂ Hu F₁ F₂ HF.
+  apply V_rel_intro; iintros u1 u2 Hu F1 F2 HF.
   eapply Obs_red_both; [ auto_red | auto_red | ]; later_shift; term_simpl.
   eapply Obs_red_both; [ auto_red | auto_red | ]; later_shift; term_simpl.
   apply K_rel_elim; assumption.
 Qed.
 
-Lemma rel_e_compat_abort {V : Set} (p₁ p₂ : program V) n :
-  n ⊨ rel_p p₁ p₂ →
-  n ⊨ E_rel (e_abort p₁) (e_abort p₂).
+Lemma rel_e_compat_abort {V : Set} (p1 p2 : program V) n :
+  n ⊨ rel_p p1 p2 →
+  n ⊨ E_rel (e_abort p1) (e_abort p2).
 Proof.
   intro Hp.
-  iintros γ₁ γ₂ Hγ E₁ E₂ HE; term_simpl.
+  iintros γ1 γ2 Hγ E1 E2 HE; term_simpl.
   eapply Obs_red_both; [ auto_red | auto_red | ]; later_shift; term_simpl.
   iapply Hp; assumption.
 Qed. *)
@@ -493,16 +573,16 @@ Qed. *)
 Lemma rel_v_compat_var {V : Set} (x : V) n :
   n ⊨ rel_v (v_var x) (v_var x).
 Proof.
-  iintros γ₁ γ₂ Hγ; iapply Hγ.
+  iintros γ1 γ2 Hγ; iapply Hγ.
 Qed.
 
-Lemma rel_v_compat_lam {V : Set} (e₁ e₂ : expr (inc V)) n :
-  n ⊨ E_rel e₁ e₂ →
-  n ⊨ rel_v (v_lam e₁) (v_lam e₂).
+Lemma rel_v_compat_lam {V : Set} (e1 e2 : expr (inc V)) n :
+  n ⊨ E_rel e1 e2 →
+  n ⊨ rel_v (v_lam e1) (v_lam e2).
 Proof.
   intro He;
-  iintros γ₁ γ₂ Hγ; term_simpl.
-  apply V_rel_intro; iintros u₁ u₂ Hu.
+  iintros γ1 γ2 Hγ; term_simpl.
+  apply V_rel_intro; iintros u1 u2 Hu.
   eapply R_rel_red_both; [ auto_red | auto_red | ]; later_shift; term_simpl.
   unfold subst; repeat rewrite bind_bind_comp'.
   iapply He.
@@ -514,15 +594,15 @@ Qed.
 (* ========================================================================= *)
 (* programs *)
 
-Lemma rel_p_compat_expr {V : Set} (e₁ e₂ : expr V) n :
-  n ⊨ E_rel e₁ e₂ →
-  n ⊨ rel_p e₁ e₂.
+Lemma rel_p_compat_expr {V : Set} (e1 e2 : expr V) n :
+  n ⊨ E_rel e1 e2 →
+  n ⊨ rel_p e1 e2.
 Proof.
   intro He.
-  iintros γ₁ γ₂ Hγ; term_simpl.
-  apply E_rel_elim with (E₁ := ectx_hole) (E₂ := ectx_hole).
+  iintros γ1 γ2 Hγ; term_simpl.
+  apply E_rel_elim with (E1 := ectx_hole) (E2 := ectx_hole).
   + iapply He; assumption.
-  + apply K_rel_intro; iintros v₁ v₂ Hv; apply Obs_value.
+  + apply K_rel_intro; iintros v1 v2 Hv; apply Obs_value.
 Qed.
 
 Fixpoint fundamental_property_e {V : Set} (e : expr V) n :
@@ -543,239 +623,3 @@ Proof.
 + destruct p.
   - apply rel_p_compat_expr, fundamental_property_e.
 Qed.
-
-(* Definition F_ObsL (ObsL : Obs_sig) : Obs_sig :=
-  λ p₁ p₂,
-  (∀ v₁ : val, p₁ = v₁ → terminates p₂)ᵢ ∧ᵢ
-  ∀ᵢ p₁' : program ∅, (red p₁ p₁')ᵢ →ᵢ ▷ ObsL p₁' p₂. *)
-
-(*
-
-Definition O_rel_pre (L_rel:expr_rel) : expr_rel :=
-  mk_expr_rel (fun e =>
-    (L_rel (e.1, e.2) ∧ L_rel (e.2, e.1))%I).
-
-Instance L_rel_pre_contractive :
-  Contractive L_rel_pre.
-Proof. solve_contractive. Qed.
-
-Definition L_rel : expr_rel := fixpoint L_rel_pre.
-Definition O_rel : expr_rel := O_rel_pre L_rel.
-
-Definition K_rel_pre (V_rel:val_rel) : evctx_rel :=
-  mk_evctx_rel (fun E =>
-    ∀ (v1 v2:val), □ (V_rel (v1, v2) →
-      O_rel (fill E.1 (of_val v1), fill E.2 (of_val v2))))%I.
-
-Definition R_rel_pre (V_rel:val_rel) : expr_rel :=
-  mk_expr_rel (fun e =>
-    ∀ (E1 E2:ectx), □ (▷ K_rel_pre V_rel (E1, E2) →
-      O_rel (fill E1 e.1, fill E2 e.2)))%I.
-
-Definition V_rel_pre (V_rel:val_rel) : val_rel :=
-  mk_val_rel (fun v =>
-    ∀ (v1' v2':val), □ (▷ V_rel (v1', v2') →
-      R_rel_pre V_rel (app (of_val v.1) (of_val v1'),
-        app (of_val v.2) (of_val v2'))))%I.
-
-Instance V_rel_pre_contractive :
-  Contractive (V_rel_pre).
-Proof. solve_contractive. Qed.
-
-Definition V_rel : val_rel := fixpoint V_rel_pre.
-Definition K_rel : evctx_rel := K_rel_pre V_rel.
-Definition R_rel : expr_rel := R_rel_pre V_rel.
-
-Definition E_rel : expr_rel :=
-  mk_expr_rel (fun e =>
-    ∀ (E1 E2:ectx), □ (K_rel (E1, E2) →
-      O_rel (fill E1 e.1, fill E2 e.2)))%I.
-
-(* open relations *)
-
-(* Definition subO := leibnizO sub. *)
-(* Definition sub_rel := subO -n> subO -n> iProp Σ. *)
-
-Definition sub_rel := persistent_pred (sub * sub) (iPropI Σ).
-Definition sub_relO := persistent_predO (sub * sub) (iPropI Σ).
-
-Definition mk_sub_rel (pred : (sub * sub) → iProp Σ) {Pers : ∀ g, Persistent (pred g)} : sub_rel :=
-  @PersPred _ _ pred Pers.
-Global Instance sub_rel_pers (τ : sub_relO) : ∀ g, Persistent (τ g) := _.
-
-
-Definition G_rel : sub_rel :=
-  mk_sub_rel (fun g =>
-    ∀ x v1 v2,
-      ⌜g.1 !! x = Some v1⌝ →
-      ⌜g.2 !! x = Some v2⌝ →
-      V_rel (v1, v2))%I.
-
-(* relations for open terms *)
-Definition E_rel_o : expr_rel :=
-  mk_expr_rel (fun e =>
-    ∀ (g1 g2:sub), □ (G_rel (g1, g2) →
-      E_rel (subst_map g1 e.1, subst_map g2 e.2)))%I.
-
-Definition O_rel_o : expr_rel :=
-  mk_expr_rel (fun e =>
-    ∀ (g1 g2:sub),
-      □ (G_rel (g1, g2) →
-        O_rel (subst_map g1 e.1, subst_map g2 e.2)))%I.
-
-(* Definition V_rel_o : val_rel :=
-  mk_val_rel (fun v =>
-    (∀ (g1 g2:sub) (v1' v2':val),
-      ⌜to_val (subst_map g1 (of_val v.1)) = Some v1'⌝ →
-      ⌜to_val (subst_map g2 (of_val v.2)) = Some v2'⌝ →
-      V_rel (v1', v2')))%I. *)
-
-Definition V_rel_o : val_rel :=
-  mk_val_rel (fun v =>
-    (∀ (g1 g2:sub),
-      V_rel (subst_map_val g1 v.1, subst_map_val g2 v.2)))%I.
-
-(* compatibility lemmas *)
-
-(* TODO it should possible to prevent iris from "leaking out" here,
-  so it is only used to define these things *)
-Lemma erel_to_vrel e1 e2 v1 v2:
-  ⊢ E_rel_o (e1, e2) →
-    ⌜to_val e1 = Some v1⌝ →
-    ⌜to_val e2 = Some v2⌝ →
-    V_rel_o (v1, v2)%I.
-Proof.
-Admitted.
-
-Lemma K_rel_elim (E1 E2 : ectx) (v1 v2 : val) :
-  (⊢ K_rel (E1, E2)) →
-  (⊢ V_rel (v1, v2)) →
-  ⊢ O_rel (fill E1 (of_val v1), fill E2 (of_val v2)).
-Proof.
-  intros HE Hv.
-  (* unfold K_rel, K_rel_pre in HE. simpl in HE. *)
-  (* unfold O_rel, O_rel_pre. simpl. *)
-  iApply HE.
-  iApply Hv.
-Qed.
-
-Lemma K_rel_elim1 (E1 E2 : ectx) (v1 v2 : val) :
-  K_rel (E1, E2) ∧ V_rel (v1, v2)
-  ⊢ O_rel (fill E1 (of_val v1), fill E2 (of_val v2)).
-Proof.
-  iIntros "[#HE #Hv]".
-  (* intros HE Hv. *)
-  (* unfold K_rel, K_rel_pre in HE. simpl in HE. *)
-  (* unfold O_rel, O_rel_pre. simpl. *)
-  iApply "HE".
-  iApply "Hv".
-Qed.
-
-(* Search (⊢ _ → _). *)
-(* Check bi.entails_impl. *)
-(* Check bi.impl_entails. *)
-
-(* aka val_inclusion *)
-Theorem compat_val: ∀ v1 v2,
-  V_rel_o (v1, v2)
-  ⊢ E_rel_o (of_val v1, of_val v2).
-Proof.
-  (* intros * Hv. *)
-  iIntros "%v1 %v2 #Hv".
-  Opaque E_rel.
-  Opaque V_rel_o.
-  Opaque G_rel.
-  unfold E_rel_o. simpl.
-  iIntros "%g1 %g2". iModIntro. iIntros "#H".
-  Transparent E_rel.
-  unfold E_rel.
-  Opaque O_rel.
-  Opaque K_rel.
-  simpl.
-  iIntros "%E1 %E2".
-  iModIntro.
-  iIntros "#HK".
-
-  (* iApply "Hv". *)
-
-  (* Check K_rel_elim1. *)
-  (* iUnfold V_rel_o in "Hv". *)
-
-  (* iPoseProof (K_rel_elim1 $! E1 E2 with "[HE]") as "H1". *)
- (* g2 v1 v2 with "HE" *)
-  (* iAssert K_rel_elim as "H1". *)
-  (* iSpecialize (K_rel_elim). *)
-
-  iApply K_rel_elim1.
-  iSplit.
-  - iApply "HK".
-  -
-  iApply "Hv".
-Qed.
-
-
-Theorem compat_var: ∀ x,
-  ⊢ E_rel_o (var x, var x).
-Proof.
-Admitted.
-
-Theorem compat_app: ∀ e1 e2 e1' e2',
-  E_rel_o (e1, e2) ∧
-  E_rel_o (e1', e2')
-  ⊢ E_rel_o (app e1 e1', app e2 e2').
-Proof.
-Admitted.
-
-Theorem compat_abs: ∀ e1 e2 x,
-  E_rel_o (e1, e2)
-  ⊢ V_rel_o (vlambda x e1, vlambda x e2).
-Proof.
-Admitted.
-
-Theorem compat_plus: ∀ e1 e2,
-  E_rel_o (e1, e1) ∧
-  E_rel_o (e2, e2)
-  ⊢ E_rel_o (eplus e1 e2, eplus e1 e2).
-Proof.
-Admitted.
-
-Fixpoint fundmental_e e:
-  ⊢ E_rel_o (e, e)
-with fundmental_v v:
-  ⊢ V_rel_o (v, v).
-Proof.
-  { induction e.
-    - pose proof (compat_val v v).
-      eauto.
-    - apply compat_var.
-    - iApply compat_app. iSplit; auto.
-    - iApply compat_plus. iSplit; auto.
-  }
-  { (* value *)
-    admit.
-  }
-Abort.
-
-Theorem L_adequacy: ∀ e1 e2,
-  L_rel (e1, e2)
-  ⊢ ⌜equiterminate e1 e2⌝.
-Proof.
-Abort.
-
-Theorem O_adequacy: ∀ e1 e2,
-  O_rel (e1, e2)
-  ⊢ ⌜equiterminate e1 e2⌝.
-Proof.
-Abort.
-
-Theorem soundness: ∀ e1 e2,
-  E_rel_o (e1, e2) ⊢ ⌜obs_eqv e1 e2⌝.
-Proof.
-Abort.
-
-Theorem completeness: ∀ e1 e2,
-  ⌜obs_eqv e1 e2⌝ ⊢ E_rel_o (e1, e2).
-Proof.
-Abort.
-
-End logrel. *)
